{
  "@context": {
    "iot": "http://iotschema.org/",
    "owl": "http://www.w3.org/2002/07/owl#",
    "qudt": "http://qudt.org/1.1/schema/qudt#",
    "rdf": "http://www.w3.org/1999/02/22-rdf-syntax-ns#",
    "rdfs": "http://www.w3.org/2000/01/rdf-schema#",
    "schema": "http://schema.org/",
    "xsd": "http://www.w3.org/2001/XMLSchema#",
	"dct": "http://purl.org/dc/terms/"
  },
  "@graph": [
    {
		"@id": "iot:TemperatureUnit",
		"@type": "rdfs:Class",
		"rdfs:comment": "An enumeration of temperature units.",
		"rdfs:label": "TemperatureUnit",
		"rdfs:subClassOf": {
			"@id": "schema:Enumeration"
		}
	},
    {
		"@id": "iot:Celsius",
		"@type": "iot:TemperatureUnit",
		"rdfs:comment": "unit of the temperature of which the scale is defined by two fixe-points, the temperatures of freezing and boiling point of water at normal pressure (air pressure of 1 013,25 hPa)",
		"rdfs:label": "Celsius",
		"iot:reference": "0112/2///62720#UAA033#001",
		"dct:source": "http://data.nasa.gov/qudt/owl/unit#DegreeCelsius"
	},
    {
		"@id": "iot:Kelvin",
		"@type": "iot:TemperatureUnit",
		"rdfs:comment": "unit of thermodynamic temperature is the fraction 1/273,16 of the thermodynamic temperature of the triple point of water",
		"rdfs:label": "Kelvin",
		"iot:reference" : "0112/2///62720#UAA185#001",
		"dct:source": "http://data.nasa.gov/qudt/owl/unit#Kelvin"
    },
	{
		"@id": "iot:Fahrenheit",
		"@type": "iot:TemperatureUnit",
		"rdfs:comment": "unit of temperature according to the temperature of the freezing and boiling point of water (32 °F and 212 °F)",
		"rdfs:label": "Fahrenheit",
		"iot:reference" : "0112/2///62720#UAA039#001",
		"dct:source": "http://data.nasa.gov/qudt/owl/unit#DegreeFahrenheit"
    },
	{
		"@id": "iot:TimeUnit",
		"@type": "rdfs:Class",
		"rdfs:comment": "An enumeration of time unit.",
		"rdfs:label": "TimeUnit",
		"rdfs:subClassOf": {
			"@id": "schema:Enumeration"
		}
	},
    {
		"@id": "iot:Second",
		"@type": "iot:TimeUnit",
		"rdfs:comment": "Second Time Unit",
		"rdfs:label": "Second",
	    "iot:reference" : "0112/2///62720#UAA972#001",
	    "dct:source": "http://data.nasa.gov/qudt/owl/unit#SecondTime"
	},
	{
		"@id": "iot:Millisecond",
		"@type": "iot:TimeUnit",
		"rdfs:comment": "Millisecond Time Unit",
		"rdfs:label": "Millisecond",
	    "iot:reference" : "0112/2///62720#UAA899",
	    "dct:source": "http://qudt.org/vocab/unit/MilliSEC"
	},
    {
		"@id": "iot:Minute",
		"@type": "iot:TimeUnit",
		"rdfs:comment": "Minute Time Unit",
		"rdfs:label": "Minute",
	    "iot:reference" : "0112/2///62720#UAA842#001",
	    "dct:source": "http://data.nasa.gov/qudt/owl/unit#MinuteTime"
	},
    {
		"@id": "iot:Hour",
		"@type": "iot:TimeUnit",
		"rdfs:comment": "Hour Time Unit",
		"rdfs:label": "Hour",
	    "iot:reference" : "0112/2///62720#UAA407#001",
	    "dct:source": "http://data.nasa.gov/qudt/owl/unit#Hour"
	},
    {
		"@id": "iot:Lux",
		"@type": "iot:IlluminanceUnit",
		"rdfs:comment": "Illuminance Unit",
		"rdfs:label": "Lux",
	    "iot:reference" : "0112/2///62720#UAA723#001",
	    "dct:source": "http://qudt.org/vocab/unit#Lux"
	},
	{
		"@id": "iot:LevelUnit",
		"@type": "rdfs:Class",
		"rdfs:comment": "An enumeration of level units.",
		"rdfs:label": "LevelUnit",
		"rdfs:subClassOf": {
		"@id": "schema:Enumeration"
		}
	},
	{
		"@id": "iot:Percent",
		"@type": "iot:LevelUnit",
		"@type": "iot:GasInAirConcentrationUnit",
		"rdfs:comment": "Unit of measurement for level or concentration.",
		"rdfs:label": "Percent",
	    "iot:reference" : "0112/2///62720#UAA000#001",
	    "dct:source": "http://qudt.org/vocab/unit#Percent"
	},
    {
		"@id": "iot:Millimetre",
		"@type": "iot:LevelUnit",
		"rdfs:comment": "Unit of measurement in millimetre",
		"rdfs:label": "Millimetre",
	    "iot:reference" : "0112/2///62720#UAA862#001"
	},
    {
		"@id": "iot:Centimetre",
		"@type": "iot:LevelUnit",
		"rdfs:comment": "Unit of measurement in centimetre",
		"rdfs:label": "Centimetre",
	    "iot:reference" : "0112/2///62720#UAA375#001",
	    "dct:source": "http://qudt.org/vocab/unit#Centimeter"
	},
	{
		"@id": "iot:DensityUnit",
		"@type": "rdfs:Class",
		"rdfs:comment": "An enumeration of density units.",
		"rdfs:label": "DensityUnit",
		"rdfs:subClassOf": {
		"@id": "schema:Enumeration"
		}
	},
    {
		"@id": "iot:KilogramPerCubicMeter",
		"@type": "iot:DensityUnit",
		"rdfs:comment": "unit of the density of liquid",
		"rdfs:label": "KilogramPerCubicMeter",
		"iot:reference": "0112/2///62720#UAA619#001",
		"dct:source": "http://data.nasa.gov/qudt/owl/unit#KilogramPerCubicMeter"
	},
    {
		"@id": "iot:PressureUnit",
		"@type": "rdfs:Class",
		"rdfs:comment": "An enumeration of pressure units.",
		"rdfs:label": "PressureUnit",
		"rdfs:subClassOf": {
		"@id": "schema:Enumeration"
		}
	},
    {
		"@id": "iot:Pascal",
		"@type": "iot:PressureUnit",
		"rdfs:comment": "The pascal (symbol: Pa) is the SI derived unit of pressure used to quantify internal pressure, stress, Young's modulus and ultimate tensile strength. It is defined as one newton per square metre.",
		"rdfs:label": "Pascal",
		"iot:reference": "0112/2///62720#UAA258#001",
		"dct:source": "http://data.nasa.gov/qudt/owl/unit#Pascal"
	},
    {
		"@id": "iot:Bar",
		"@type": "iot:PressureUnit",
		"rdfs:comment": "The bar (symbol: bar) is a metric unit of pressure, but is not approved as part of the International System of Units (SI).",
		"rdfs:label": "Bar",
		"iot:reference": "0112/2///62720#UAA323#001",
		"dct:source": "http://data.nasa.gov/qudt/owl/unit#Bar"
	},
    {
		"@id": "iot:FlowRateUnit",
		"@type": "rdfs:Class",
		"rdfs:comment": "An enumeration of flow rate units.",
		"rdfs:label": "FlowRateUnit",
		"rdfs:subClassOf": {
		"@id": "schema:Enumeration"
		}
	},
    {
		"@id": "iot:GallonsPerMinute",
		"@type": "iot:FlowRateUnit",
		"rdfs:comment": "unit of measurement of liquid flow rate",
		"rdfs:label": "GallonsPerMinute",
		"dct:source":"http://data.nasa.gov/qudt/owl/unit#GallonUSPerMinute"
	},
    {
		"@id": "iot:LitrePerMinute",
		"@type": "iot:FlowRateUnit",
		"rdfs:comment": "Unit of measurement of flow rate of a substance",
		"rdfs:label": "LitrePerMinute",
		"iot:reference": "0112/2///62720#UAA659#001"
	},
	{
		"@id": "iot:Decibel",
		"@type": "iot:SoundPressureUnit",
		"rdfs:comment": "Sound Pressure Unit",
		"rdfs:label": "SoundPressureUnit",
		"iot:reference" : "0112/2///62720#UAA409#001",
		"dct:source": "http://qudt.org/vocab/unit#Decibel"
	},
	{
		"@id": "iot:GasInAirConcentrationUnit",
		"@type": "rdfs:Class",
		"rdfs:comment": "An enumeration of units for concentration of gas in the air, e.g., concentration of carbon dioxide (CO2) in ambient air.",
		"rdfs:label": "GasInAirConcentrationUnit",
		"rdfs:subClassOf": {
		"@id": "schema:Enumeration"
		}
	},
	{
		"@id": "iot:PartsPerMillion",
		"@type": "iot:GasInAirConcentrationUnit",
		"rdfs:comment": "The unit of concentration of gas in the air, e.g., concentration of carbon dioxide (CO2) in ambient air.",
		"rdfs:label": "parts-per-million"
	},	
	{
		"@id": "iot:ApparentPowerUnit",
		"@type": "rdfs:Class",
		"rdfs:comment": "An enumeration of apparent power units.",
		"rdfs:label": "ApparentPowerUnit",
		"rdfs:subClassOf": {
		"@id": "schema:Enumeration"
		}
	},
	{
		"@id": "iot:VoltAmpere",
		"@type": "iot:ApparentPowerUnit",
		"rdfs:comment": "The unit of the apparent power.",
		"rdfs:label": "volt-ampere",
		"iot:reference": "0112/2///62720#UAA298#001"
	},
	{
		"@id": "iot:KiloVoltAmpere",
		"@type": "iot:ApparentPowerUnit",
		"rdfs:comment": "The unit of the apparent power, expressed in kilo (one thousand) as a decimal unit prefix.",
		"rdfs:label": "kilovolt-ampere",
		"iot:reference": "0112/2///62720#UAA581#001"
	},
	{
		"@id": "iot:MegaVoltAmpere",
		"@type": "iot:ApparentPowerUnit",
		"rdfs:comment": "The unit of the apparent power, expressed in mega (one million) as a decimal unit prefix.",
		"rdfs:label": "megavolt-ampere",
		"iot:reference": "0112/2///62720#UAA222#001"
	},
	{
		"@id": "iot:GigaVoltAmpere",
		"@type": "iot:ApparentPowerUnit",
		"rdfs:comment": "The unit of the apparent power, expressed in giga (one billion) as a decimal unit prefix.",
		"rdfs:label": "gigavolt-ampere", 
		"iot:reference": "0112/2///62720#UAB534#001"
	},
	{
		"@id": "iot:ActivePowerUnit",
		"@type": "rdfs:Class",
		"rdfs:comment": "An enumeration of active power units.",
		"rdfs:label": "ActivePowerUnit",
		"rdfs:subClassOf": {
		"@id": "schema:Enumeration"
		}
	},
	{
		"@id": "iot:Watt",
		"@type": "iot:ActivePowerUnit",
		"rdfs:comment": "The unit of the active power.",
		"rdfs:label": "watt",
		"dct:source": "http://www.qudt.org/qudt/owl/1.0.0/unit/Instances.html#Watt",
		"iot:reference": "0112/2///62720#UAA306#001"
	},
	{
		"@id": "iot:KiloWatt",
		"@type": "iot:ActivePowerUnit",
		"rdfs:comment": "The unit of the active power, expressed in kilo (one thousand) as a decimal unit prefix.",
		"rdfs:label": "kilowatt",
		"iot:reference": "0112/2///62720#UAA583#001"
	},
	{
		"@id": "iot:MegaWatt",
		"@type": "iot:ActivePowerUnit",
		"rdfs:comment": "The unit of the active power, expressed in mega (one million) as a decimal unit prefix.",
		"rdfs:label": "megawatt",
		"iot:reference": "0112/2///62720#UAA224#001"
	},
	{
		"@id": "iot:GigaWatt",
		"@type": "iot:ActivePowerUnit",
		"rdfs:comment": "The unit of the active power, expressed in giga (one billion) as a decimal unit prefix.",
		"rdfs:label": "gigawatt",
		"iot:reference": "0112/2///62720#UAA154#001"
	},
	{
		"@id": "iot:ReactivePowerUnit",
		"@type": "rdfs:Class",
		"rdfs:comment": "An enumeration of reactive power units.",
		"rdfs:label": "ReactivePowerUnit",
		"rdfs:subClassOf": {
		"@id": "schema:Enumeration"
		}
	},
	{
		"@id": "iot:VoltAmpereReactive",
		"@type": "iot:ReactivePowerUnit",
		"rdfs:comment": "The unit of reactive power.",
		"rdfs:label": "volt-ampere-reactive",
		"iot:reference": "0112/2///62720#UAB023#001"
	},
	{
		"@id": "iot:KiloVoltAmpereReactive",
		"@type": "iot:ReactivePowerUnit",
		"rdfs:comment": "The unit of reactive power, expressed in kilo (one thousand) as a decimal unit prefix.",
		"rdfs:label": "kilovolt-ampere-reactive",
		"iot:reference": "0112/2///62720#UAB195#001"
	},
	{
		"@id": "iot:MegaVoltAmpereReactive",
		"@type": "iot:ReactivePowerUnit",
		"rdfs:comment": "The unit of reactive power, expressed in mega (one million) as a decimal unit prefix.",
		"rdfs:label": "megavolt-ampere-reactive",
		"iot:reference": "0112/2///62720#UAB199#001"
	},
	{
		"@id": "iot:GigaVoltAmpereReactive",
		"@type": "iot:ReactivePowerUnit",
		"rdfs:comment": "The unit of reactive power, expressed in giga (one billion) as a decimal unit prefix.",
		"rdfs:label": "gigavolt-ampere-reactive"
	},	
	{
		"@id": "iot:ElectricCurrentUnit",
		"@type": "rdfs:Class",
		"rdfs:comment": "An enumeration of electric current units.",
		"rdfs:label": "ElectricCurrentUnit",
		"rdfs:subClassOf": {
		"@id": "schema:Enumeration"
		}
	},
	{
		"@id": "iot:Ampere",
		"@type": "iot:ElectricCurrentUnit",
		"rdfs:comment": "The unit of electric current.",
		"rdfs:label": "ampere",
		"iot:reference": "0112/2///62720#UAA101#001",
		"dct:source": "http://www.qudt.org/qudt/owl/1.0.0/unit/Instances.html#Ampere"
	},
	{
		"@id": "iot:FemtoAmpere",
		"@type": "iot:ElectricCurrentUnit",
		"rdfs:comment": "The unit of electric current, expressed in a unit prefix meaning 'one 0.000000000000001'.",
		"rdfs:label": "femtoampere",
		"iot:reference": "0112/2///62720#UAB638#001"
	},
	{
		"@id": "iot:PicoAmpere",
		"@type": "iot:ElectricCurrentUnit",
		"rdfs:comment": "The unit of electric current, expressed in a unit prefix meaning 'one trillionth'.",
		"rdfs:label": "picoampere",
		"iot:reference": "0112/2///62720#UAA928#001"
	},
	{
		"@id": "iot:NanoAmpere",
		"@type": "iot:ElectricCurrentUnit",
		"rdfs:comment": "The unit of electric current, expressed in a unit prefix meaning 'one billionth'.",
		"rdfs:label": "nanoampere",
		"iot:reference": "0112/2///62720#UAA901#001"
	},
	{
		"@id": "iot:MicroAmpere",
		"@type": "iot:ElectricCurrentUnit",
		"rdfs:comment": "The unit of electric current, expressed in a unit prefix meaning 'one millionth'.",
		"rdfs:label": "microampere",
		"iot:reference": "0112/2///62720#UAA057#001"
	},
	{
		"@id": "iot:MilliAmpere",
		"@type": "iot:ElectricCurrentUnit",
		"rdfs:comment": "The unit of electric current, expressed in a unit prefix meaning 'one thousandth'.",
		"rdfs:label": "milliampere",
		"iot:reference": "0112/2///62720#UAA775#001"
	},
	{
		"@id": "iot:KiloAmpere",
		"@type": "iot:ElectricCurrentUnit",
		"rdfs:comment": "The unit of electric current, expressed in a unit prefix meaning 'one thousand'.",
		"rdfs:label": "kiloampere",
		"iot:reference": "0112/2///62720#UAA557#001"
	},
	{
		"@id": "iot:MegaAmpere",
		"@type": "iot:ElectricCurrentUnit",
		"rdfs:comment": "The unit of electric current, expressed in a unit prefix meaning 'one million'.",
		"rdfs:label": "megaampere",
		"iot:reference": "0112/2///62720#UAA202#001"
	},
	{
		"@id": "iot:GigaAmpere",
		"@type": "iot:ElectricCurrentUnit",
		"rdfs:comment": "The unit of electric current, expressed in a unit prefix meaning 'one billion'.",
		"rdfs:label": "gigaampere"
	},
	{
		"@id": "iot:TeraAmpere",
		"@type": "iot:ElectricCurrentUnit",
		"rdfs:comment": "The unit of electric current, expressed in a unit prefix meaning 'one trillion'.",
		"rdfs:label": "teraampere",
		"iot:reference": "0112/2///62720#UAB640#001"
	},	
	{
		"@id": "iot:LineFrequencyUnit",
		"@type": "rdfs:Class",
		"rdfs:comment": "An enumeration of line frequency units.",
		"rdfs:label": "LineFrequencyUnit",
		"rdfs:subClassOf": {
		"@id": "schema:Enumeration"
		}
	},
	{
		"@id": "iot:Hertz",
		"@type": "iot:LineFrequencyUnit",
		"rdfs:comment": "The unit of line frequency.",
		"rdfs:label": "hertz",
		"iot:reference": "0112/2///62720#UAA170#001",
		"dct:source": "http://www.qudt.org/qudt/owl/1.0.0/unit/Instances.html#Hertz"
	},
	{
		"@id": "iot:Femtohertz",
		"@type": "iot:LineFrequencyUnit",
		"rdfs:comment": "The unit of line frequency, expressed in a unit prefix meaning 'one 0.000000000000001'.",
		"rdfs:label": "femtohertz"
	},
	{
		"@id": "iot:Picohertz",
		"@type": "iot:LineFrequencyUnit",
		"rdfs:comment": "The unit of line frequency, expressed in a unit prefix meaning 'one trillionth'.",
		"rdfs:label": "picohertz"
	},
	{
		"@id": "iot:Nanoampere",
		"@type": "iot:LineFrequencyUnit",
		"rdfs:comment": "The unit of line frequency, expressed in a unit prefix meaning 'one billionth'.",
		"rdfs:label": "nanohertz"
	},
	{
		"@id": "iot:Microhertz",
		"@type": "iot:LineFrequencyUnit",
		"rdfs:comment": "The unit of line frequency, expressed in a unit prefix meaning 'one millionth'.",
		"rdfs:label": "microhertz"
	},
	{
		"@id": "iot:Millihertz",
		"@type": "iot:LineFrequencyUnit",
		"rdfs:comment": "The unit of line frequency, expressed in a unit prefix meaning 'one thousandth'.",
		"rdfs:label": "millihertz",
		"iot:reference": "0112/2///62720#UAB698#001"
	},
	{
		"@id": "iot:KiloHertz",
		"@type": "iot:LineFrequencyUnit",
		"rdfs:comment": "The unit of line frequency, expressed in a unit prefix meaning 'one thousand'.",
		"rdfs:label": "kilohertz",
		"iot:reference": "0112/2///62720#UAA566#001",
		"dct:source": "http://www.qudt.org/qudt/owl/1.0.0/unit/Instances.html#KiloHertz"
	},
	{
		"@id": "iot:MegaHertz",
		"@type": "iot:LineFrequencyUnit",
		"rdfs:comment": "The unit of line frequency, expressed in a unit prefix meaning 'one million'.",
		"rdfs:label": "megahertz",
		"iot:reference": "0112/2///62720#UAA209#001",
		"dct:source": "http://www.qudt.org/qudt/owl/1.0.0/unit/Instances.html#MegaHertz"
	},
	{
		"@id": "iot:GigaHertz",
		"@type": "iot:LineFrequencyUnit",
		"rdfs:comment": "The unit of line frequency, expressed in a unit prefix meaning 'one billion'.",
		"rdfs:label": "gigahertz",
		"iot:reference": "0112/2///62720#UAA150#001",
		"dct:source": "http://www.qudt.org/qudt/owl/1.0.0/unit/Instances.html#GigaHertz"
	},
	{
		"@id": "iot:TeraHertz",
		"@type": "iot:LineFrequencyUnit",
		"rdfs:comment": "The unit of line frequency, expressed in a unit prefix meaning 'one trillion'.",
		"rdfs:label": "terahertz",
		"iot:reference": "0112/2///62720#UAA287#001"
	},	
	{
		"@id": "iot:VoltageUnit",
		"@type": "rdfs:Class",
		"rdfs:comment": "An enumeration of voltage units.",
		"rdfs:label": "VoltageUnit",
		"rdfs:subClassOf": {
		"@id": "schema:Enumeration"
		}
	},
	{
		"@id": "iot:Volt",
		"@type": "iot:VoltageUnit",
		"rdfs:comment": "The unit of voltage.",
		"rdfs:label": "volt",
		"iot:reference": "0112/2///62720#UAA296#001",
		"dct:source": "http://www.qudt.org/qudt/owl/1.0.0/unit/Instances.html#Volt"
	},
	{
		"@id": "iot:FemtoVolt",
		"@type": "iot:VoltageUnit",
		"rdfs:comment": "The unit of voltage, expressed in a unit prefix meaning 'one 0.000000000000001'.",
		"rdfs:label": "femtovolt",
		"iot:reference": "0112/2///62720#UAC770#001"
	},
	{
		"@id": "iot:PicoVolt",
		"@type": "iot:VoltageUnit",
		"rdfs:comment": "The unit of voltage, expressed in a unit prefix meaning 'one trillionth'.",
		"rdfs:label": "picovolt",
		"iot:reference": "0112/2///62720#UAB363#001"
	},
	{
		"@id": "iot:NanoVolt",
		"@type": "iot:VoltageUnit",
		"rdfs:comment": "The unit of voltage, expressed in a unit prefix meaning 'one billionth'.",
		"rdfs:label": "nanovolt",
		"iot:reference": "0112/2///62720#UAC771#001"
	},
	{
		"@id": "iot:MicroVolt",
		"@type": "iot:VoltageUnit",
		"rdfs:comment": "The unit of voltage, expressed in a unit prefix meaning 'one millionth'.",
		"rdfs:label": "microvolt",
		"iot:reference": "0112/2///62720#UAA078#001"
	},
	{
		"@id": "iot:MilliVolt",
		"@type": "iot:VoltageUnit",
		"rdfs:comment": "The unit of voltage, expressed in a unit prefix meaning 'one thousandth'.",
		"rdfs:label": "millivolt",
		"iot:reference": "0112/2///62720#UAA804#001"
	},
	{
		"@id": "iot:KiloVolt",
		"@type": "iot:VoltageUnit",
		"rdfs:comment": "The unit of voltage, expressed in a unit prefix meaning 'one thousand'.",
		"rdfs:label": "kilovolt",
		"iot:reference": "0112/2///62720#UAA580#001"
	},
	{
		"@id": "iot:MegaVolt",
		"@type": "iot:VoltageUnit",
		"rdfs:comment": "The unit of voltage, expressed in a unit prefix meaning 'one million'.",
		"rdfs:label": "megavolt",
		"iot:reference": "0112/2///62720#UAA221#001"
	},
	{
		"@id": "iot:GigaVolt",
		"@type": "iot:VoltageUnit",
		"rdfs:comment": "The unit of voltage, expressed in a unit prefix meaning 'one billion'.",
		"rdfs:label": "gigavolt",
		"iot:reference": "0112/2///62720#UAC772#001"
	},
	{
		"@id": "iot:TeraVolt",
		"@type": "iot:VoltageUnit",
		"rdfs:comment": "The unit of voltage, expressed in a unit prefix meaning 'one trillion'.",
		"rdfs:label": "teravolt",
		"iot:reference": "0112/2///62720#UAC773#001"
	},	
	{
		"@id": "iot:ApparentEnergyUnit",
		"@type": "rdfs:Class",
		"rdfs:comment": "An enumeration of apparent energy units.",
		"rdfs:label": "ApparentEnergyUnit",
		"rdfs:subClassOf": {
		"@id": "schema:Enumeration"
		}
	},
	{
		"@id": "iot:VoltAmpereHours",
		"@type": "iot:ApparentEnergyUnit",
		"rdfs:comment": "The unit of the apparent energy.",
		"rdfs:label": "volt-ampere-hours"
	},
	{
		"@id": "iot:KiloVoltAmpereHours",
		"@type": "iot:ApparentEnergyUnit",
		"rdfs:comment": "The unit of the apparent enregy, expressed in kilo (one thousand) as a decimal unit prefix.",
		"rdfs:label": "kilovolt-ampere-hours"
	},
	{
		"@id": "iot:MegaVoltAmpereHours",
		"@type": "iot:ApparentEnergyUnit",
		"rdfs:comment": "The unit of the apparent enregy, expressed in mega (one million) as a decimal unit prefix.",
		"rdfs:label": "megavolt-ampere-hours"
	},
	{
		"@id": "iot:GigaVoltAmpereHours",
		"@type": "iot:ApparentEnergyUnit",
		"rdfs:comment": "The unit of the apparent enregy, expressed in giga (one billion) as a decimal unit prefix.",
		"rdfs:label": "gigavolt-ampere-hours"
	},
	{
		"@id": "iot:TeraVoltAmpereHours",
		"@type": "iot:ApparentPowerUnit",
		"rdfs:comment": "The unit of the apparent enregy, expressed in giga (one trillion) as a decimal unit prefix.",
		"rdfs:label": "teravolt-ampere-hours"
	},
	{
		"@id": "iot:ActiveEnergyUnit",
		"@type": "rdfs:Class",
		"rdfs:comment": "An enumeration of active enregy units.",
		"rdfs:label": "ActiveEnergyUnit",
		"rdfs:subClassOf": {
		"@id": "schema:Enumeration"
		}
	},
	{
		"@id": "iot:WattHour",
		"@type": "iot:ActiveEnergyUnit",
		"rdfs:comment": "The unit of the active enregy.",
		"rdfs:label": "watt-hour",
		"dct:source": "http://www.qudt.org/qudt/owl/1.0.0/unit/Instances.html#Watthour",
		"iot:reference": "0112/2///62720#UAA308#001"
	},
	{
		"@id": "iot:KiloWattHour",
		"@type": "iot:ActiveEnergyUnit",
		"rdfs:comment": "The unit of the active enregy, expressed in kilo (one thousand) as a decimal unit prefix.",
		"rdfs:label": "kilowatt-hour",
		"dct:source": "http://www.qudt.org/qudt/owl/1.0.0/unit/Instances.html#Kilowatthour",
		"iot:reference": "0112/2///62720#UAA584#001"
	},
	{
		"@id": "iot:MegaWattHour",
		"@type": "iot:ActiveEnergyUnit",
		"rdfs:comment": "The unit of the active enregy, expressed in mega (one million) as a decimal unit prefix.",
		"rdfs:label": "megawatt-hour",
		"iot:reference": "0112/2///62720#UAA225#001"
	},
	{
		"@id": "iot:GigaWattHour",
		"@type": "iot:ActiveEnergyUnit",
		"rdfs:comment": "The unit of the active enregy, expressed in giga (one billion) as a decimal unit prefix.",
		"rdfs:label": "gigawatt-hour",
		"iot:reference": "0112/2///62720#UAA155#001"
	},
	{
		"@id": "iot:TeraWattHour",
		"@type": "iot:ActiveEnergyUnit",
		"rdfs:comment": "The unit of the active enregy, expressed in giga (one trillion) as a decimal unit prefix.",
		"rdfs:label": "terawatt-hour",
		"iot:reference": "0112/2///62720#UAA155#001"
	},
	{
		"@id": "iot:ReactiveEnergyUnit",
		"@type": "rdfs:Class",
		"rdfs:comment": "An enumeration of reactive enregy units.",
		"rdfs:label": "ReactiveEnergyUnit",
		"rdfs:subClassOf": {
		"@id": "schema:Enumeration"
		}
	},
	{
		"@id": "iot:VoltAmpereReactiveHour",
		"@type": "iot:ReactiveEnergyUnit",
		"rdfs:comment": "The unit of reactive enregy.",
		"rdfs:label": "volt-ampere-reactive-hour"
	},
	{
		"@id": "iot:KiloVoltAmpereReactiveHour",
		"@type": "iot:ReactiveEnergyUnit",
		"rdfs:comment": "The unit of reactive enregy, expressed in kilo (one thousand) as a decimal unit prefix.",
		"rdfs:label": "kilovolt-ampere-reactive-hour",
		"iot:reference": "0112/2///62720#UAB195#001"
	},
	{
		"@id": "iot:MegaVoltAmpereReactiveHour",
		"@type": "iot:ReactiveEnergyUnit",
		"rdfs:comment": "The unit of reactive enregy, expressed in mega (one million) as a decimal unit prefix.",
		"rdfs:label": "megavolt-ampere-reactive-hour",
		"iot:reference": "0112/2///62720#UAB198#001"
	},
	{
		"@id": "iot:GigaVoltAmpereReactiveHour",
		"@type": "iot:ReactiveEnergyUnit",
		"rdfs:comment": "The unit of reactive enregy, expressed in giga (one billion) as a decimal unit prefix.",
		"rdfs:label": "gigavolt-ampere-reactive-hour"
	},
	{
		"@id": "iot:TeraVoltAmpereReactiveHour",
		"@type": "iot:ReactiveEnergyUnit",
		"rdfs:comment": "The unit of the reactive enregy, expressed in giga (one trillion) as a decimal unit prefix.",
		"rdfs:label": "teravolt-ampere-reactive-hour"
	},
	{
		"@id": "iot:AmpereHour",
		"@type": "iot:ElectricChargeUnit",
		"rdfs:comment": "The unit of the electric charge (battery capacity).",
		"rdfs:label": "ampere-hour",
		"iot:reference": "0112/2///62720#UAA102#001",
		"dct:source": "http://www.qudt.org/qudt/owl/1.0.0/unit/Instances.html#AmpereHour"
	},
	{
		"@id": "iot:KiloAmpereHour",
		"@type": "iot:ElectricChargeUnit",
		"rdfs:comment": "The unit of the electric charge (battery capacity), expressed in a unit prefix meaning 'one thousand'.",
		"rdfs:label": "kilo-ampere-hour",
		"iot:reference": "0112/2///62720#UAB053#001"
	},
	{
		"@id": "iot:MilliAmpereHour",
		"@type": "iot:ElectricChargeUnit",
		"rdfs:comment": "The unit of the electric charge (battery capacity), expressed in a unit prefix meaning 'one thousandth'.",
		"rdfs:label": "milli-ampere-hour",
		"iot:reference": "0112/2///62720#UAA777#001"
	},
	{
		"@id": "iot:ReciprocalHour",
		"@type": "iot:CRateUnit",
		"rdfs:comment": "Reciprocal of the unit hour",
		"rdfs:label": "reciprocal-hour",
		"iot:reference": "0112/2///62720#UAA526#001"
	}
  ]
}
