{
    "@context" : [
	{
		"rdf": "http://www.w3.org/1999/02/22-rdf-syntax-ns#",
		"rdfs": "http://www.w3.org/2000/01/rdf-schema#",
		"schema": "http://schema.org/",
		"iot": "http://iotschema.org/"
	}],
	"@graph": [
	{
		"@id": "iot:AirConditioner",
		"@type": "rdfs:Class",
		"rdfs:subClassOf": { "@id": "iot:Capability" },
		"rdfs:comment": "A capability for air conditioner",
		"rdfs:label": "AirConditioner",
		"iot:domain": {"@id": "iot:Home"}
	},
	{
		"@id": "iot:HumiditySensing",
		"@type": "rdfs:Class",
		"rdfs:subClassOf": { "@id": "iot:Capability" },
		"rdfs:comment": "Current sensed value for humidity.",
		"rdfs:label": "HumiditySensing",
		"iot:domain": [
			{"@id": "iot:Home"},
			{"@id": "iot:Building"}
			]
	},
	{
		"@id": "iot:TemperatureSensing",
		"@type": "rdfs:Class",
		"rdfs:subClassOf": { "@id": "iot:Capability" },
		"rdfs:comment": "A capability for temperature sensing",
		"rdfs:label": "TemperatureSensing",
		"iot:domain": {"@id": "iot:Common"}
	},
	{
		"@id": "iot:Thermostat",
		"@type": "rdfs:Class",
		"rdfs:subClassOf": { "@id": "iot:Capability" },
		"rdfs:comment": "A capability for thermostat",
		"rdfs:label": "Thermostat",
		"iot:domain": {"@id": "iot:Common"}
	},
	{
		"@id": "iot:IlluminanceSensing",
		"@type": "rdfs:Class",
		"rdfs:subClassOf": { "@id": "iot:Capability" },
		"rdfs:comment": "Sensed luminous flux per unit area in lux.",
		"rdfs:label": "IlluminanceSensing",
		"iot:domain": [
			{"@id": "iot:Home"},
			{"@id": "iot:Building"}
		]
	},
	{
		"@id": "iot:MotionControl",
		"@type": "rdfs:Class",
		"rdfs:subClassOf": { "@id": "iot:Capability" },
		"rdfs:comment": "Presence (motion) sensing capability.",
		"rdfs:label": "MotionControl",
		"iot:domain": [
			{"@id": "iot:Home"},
			{"@id": "iot:Building"}
		]
	},
	{
		"@id": "iot:FloatSwitch",
		"@type": "rdfs:Class",
		"rdfs:subClassOf": { "@id": "iot:Capability" },
		"rdfs:comment": "A capability of a float switch.",
		"rdfs:label": "FloatSwitch",
		"iot:domain": {"@id": "iot:Industry"}
	},
	{
      "@id": "iot:temperature",
      "@type": "rdf:Property",
      "rdfs:label": "temperature",
	  "rdfs:comment": "A property that relates a capability with its Temperature interaction pattern.",
      "schema:domainIncludes": [
        {
          "@id": "iot:AirConditioner"
        },
        {
          "@id": "iot:TemperatureSensing"
        },
        {
          "@id": "iot:Thermostat"
        }
      ],
      "schema:rangeIncludes": {
        "@id": "iot:Temperature"
      },
	  "rdfs:subPropertyOf": {
        "@id": "iot:providesInteractionPattern"
      }
    },
	{
      "@id": "iot:targetTemperature",
      "@type": "rdf:Property",
      "rdfs:label": "targetTemperature",
	  "rdfs:comment": "A property that relates a capability with its TargetTemperature interaction pattern.",
      "schema:domainIncludes": [
        {
          "@id": "iot:AirConditioner"
        },
        {
          "@id": "iot:Thermostat"
        }
      ],
      "schema:rangeIncludes": {
        "@id": "iot:TargetTemperature"
      },
	  "rdfs:subPropertyOf": {
        "@id": "iot:providesInteractionPattern"
      }
    },
	{
      "@id": "iot:switchStatus",
      "@type": "rdf:Property",
      "rdfs:label": "switchStatus",
	  "rdfs:comment": "A property that relates a capability with its SwitchStatus interaction pattern.",
      "schema:domainIncludes": {
        "@id": "iot:AirConditioner"
      },
      "schema:rangeIncludes": {
        "@id": "iot:SwitchStatus"
      },
	  "rdfs:subPropertyOf": {
        "@id": "iot:providesInteractionPattern"
      }
    },
	{
      "@id": "iot:turnOn",
      "@type": "rdf:Property",
      "rdfs:label": "turnOn",
	  "rdfs:comment": "A property that relates a capability with its TurnOn interaction pattern.",
      "schema:domainIncludes": {
        "@id": "iot:AirConditioner"
      },
      "schema:rangeIncludes": {
        "@id": "iot:TurnOn"
      },
	  "rdfs:subPropertyOf": {
        "@id": "iot:providesInteractionPattern"
      }
    },
	{
      "@id": "iot:turnOff",
      "@type": "rdf:Property",
      "rdfs:label": "turnOff",
	  "rdfs:comment": "A property that relates a capability with its TurnOff interaction pattern.",
      "schema:domainIncludes": {
        "@id": "iot:AirConditioner"
      },
      "schema:rangeIncludes": {
        "@id": "iot:TurnOff"
      },
	  "rdfs:subPropertyOf": {
        "@id": "iot:providesInteractionPattern"
      }
    },
	{
      "@id": "iot:runMode",
      "@type": "rdf:Property",
      "rdfs:label": "runMode",
	  "rdfs:comment": "A property that relates a capability with its RunMode interaction pattern.",
      "schema:domainIncludes": {
        "@id": "iot:AirConditioner"
      },
      "schema:rangeIncludes": {
        "@id": "iot:RunMode"
      },
	  "rdfs:subPropertyOf": {
        "@id": "iot:providesInteractionPattern"
      }
    },
	{
      "@id": "iot:countDown",
      "@type": "rdf:Property",
      "rdfs:label": "countDown",
	  "rdfs:comment": "A property that relates a capability with its CountDown interaction pattern.",
      "schema:domainIncludes": {
        "@id": "iot:AirConditioner"
      },
      "schema:rangeIncludes": {
        "@id": "iot:CountDown"
      },
	  "rdfs:subPropertyOf": {
        "@id": "iot:providesInteractionPattern"
      }
    },
	{
      "@id": "iot:windStrength",
      "@type": "rdf:Property",
      "rdfs:label": "windStrength",
	  "rdfs:comment": "A property that relates a capability with its WindStrength interaction pattern.",
      "schema:domainIncludes": {
        "@id": "iot:AirConditioner"
      },
      "schema:rangeIncludes": {
        "@id": "iot:WindStrength"
      },
	  "rdfs:subPropertyOf": {
        "@id": "iot:providesInteractionPattern"
      }
    },
	{
      "@id": "iot:humidity",
      "@type": "rdf:Property",
      "rdfs:label": "humidity",
	  "rdfs:comment": "A property that relates a capability with its Humidity interaction pattern.",
      "schema:domainIncludes": [
        {
          "@id": "iot:HumiditySensing"
        }
      ],
      "schema:rangeIncludes": {
        "@id": "iot:Humidity"
      },
	  "rdfs:subPropertyOf": {
        "@id": "iot:providesInteractionPattern"
      }
    },
	{
      "@id": "iot:targetHumidity",
      "@type": "rdf:Property",
      "rdfs:label": "targetHumidity",
	  "rdfs:comment": "A property that relates a capability with its TargetHumidity interaction pattern.",
      "schema:domainIncludes": [
        {
          "@id": "iot:HumiditySensing"
        }
      ],
      "schema:rangeIncludes": {
        "@id": "iot:TargetHumidity"
      },
	  "rdfs:subPropertyOf": {
        "@id": "iot:providesInteractionPattern"
      }
    },
	  {
      "@id": "iot:illuminance",
      "@type": "rdf:Property",
      "rdfs:label": "illuminance",
	  "rdfs:comment": "A property that relates a capability with its Illuminance interaction pattern.",
      "schema:domainIncludes": [
        {
          "@id": "iot:IlluminanceSensing"
        }
      ],
      "schema:rangeIncludes": {
        "@id": "iot:Illuminance"
      },
	  "rdfs:subPropertyOf": {
        "@id": "iot:providesInteractionPattern"
      }
    },
	  {
      "@id": "iot:motionDetected",
      "@type": "rdf:Property",
      "rdfs:label": "motionDetected",
	  "rdfs:comment": "A property that relates a capability with its MotionDetected interaction pattern.",
      "schema:domainIncludes": [
        {
          "@id": "iot:MotionControl"
        }
      ],
      "schema:rangeIncludes": {
        "@id": "iot:MotionDetected"
      },
	  "rdfs:subPropertyOf": {
        "@id": "iot:providesInteractionPattern"
      }
    },
	  {
      "@id": "iot:motionType",
      "@type": "rdf:Property",
      "rdfs:label": "motionType",
	  "rdfs:comment": "A property that relates a capability with its MotionType interaction pattern.",
      "schema:domainIncludes": [
        {
          "@id": "iot:MotionControl"
        }
      ],
      "schema:rangeIncludes": {
        "@id": "iot:MotionType"
      },
	  "rdfs:subPropertyOf": {
        "@id": "iot:providesInteractionPattern"
      }
    },
	{
      "@id": "iot:overflowStatus",
      "@type": "rdf:Property",
      "rdfs:label": "overflowStatus",
	  "rdfs:comment": "A property that relates a capability with its OverflowStatus interaction pattern.",
      "schema:domainIncludes": [
        {
          "@id": "iot:FloatSwitch"
        }
      ],
      "schema:rangeIncludes": {
        "@id": "iot:OverflowStatus"
      },
	  "rdfs:subPropertyOf": {
        "@id": "iot:providesInteractionPattern"
      }
    },
	{
      "@id": "iot:expectedPressure",
      "@type": "rdf:Property",
      "rdfs:label": "expectedPressure",
	  "rdfs:comment": "A property that relates a capability with its ExpectedPressure interaction pattern.",
      "schema:domainIncludes": [
        {
          "@id": "iot:FloatSwitch"
        }
      ],
      "schema:rangeIncludes": {
        "@id": "iot:ExpectedPressure"
      },
	  "rdfs:subPropertyOf": {
        "@id": "iot:providesInteractionPattern"
      }
    },
	{
      "@id": "iot:expectedDensity",
      "@type": "rdf:Property",
      "rdfs:label": "expectedDensity",
	  "rdfs:comment": "A property that relates a capability with its ExpectedDensity interaction pattern.",
      "schema:domainIncludes": [
        {
          "@id": "iot:FloatSwitch"
        }
      ],
      "schema:rangeIncludes": {
        "@id": "iot:ExpectedDensity"
      },
	  "rdfs:subPropertyOf": {
        "@id": "iot:providesInteractionPattern"
      }
    },
	{
      "@id": "iot:expectedAmbientTemperature",
      "@type": "rdf:Property",
      "rdfs:label": "expectedAmbientTemperature",
	  "rdfs:comment": "A property that relates a capability with its ExpectedAmbientTemperature interaction pattern.",
      "schema:domainIncludes": [
        {
          "@id": "iot:FloatSwitch"
        }
      ],
      "schema:rangeIncludes": {
        "@id": "iot:ExpectedAmbientTemperature"
      },
	  "rdfs:subPropertyOf": {
        "@id": "iot:providesInteractionPattern"
      }
    },
	{
      "@id": "iot:expectedFloatImmersionDepth",
      "@type": "rdf:Property",
      "rdfs:label": "expectedFloatImmersionDepth",
	  "rdfs:comment": "A property that relates a capability with its ExpectedFloatImmersionDepth interaction pattern.",
      "schema:domainIncludes": [
        {
          "@id": "iot:FloatSwitch"
        }
      ],
      "schema:rangeIncludes": {
        "@id": "iot:ExpectedFloatImmersionDepth"
      },
	  "rdfs:subPropertyOf": {
        "@id": "iot:providesInteractionPattern"
      }
    }
	]
}
